\documentclass[12pt]{article}
\usepackage[margin=1in]{geometry}
\usepackage{parskip}
\usepackage{amsmath}

\title{Problem 3}
\author{}
\date{}

\begin{document}
\maketitle
\thispagestyle{empty}

Given data points \( (x_1, y_1), \dots, (x_m, y_m) \), we define the design matrix:
\[
X = 
\begin{bmatrix}
x_1 & 1 \\
x_2 & 1 \\
\vdots & \vdots \\
x_m & 1 \\
\end{bmatrix},
\quad
\theta = 
\begin{bmatrix}
a \\
b \\
\end{bmatrix},
\quad
y = 
\begin{bmatrix}
y_1 \\
y_2 \\
\vdots \\
y_m \\
\end{bmatrix}
\]

The normal equation for linear regression is given by:
\[
\theta = (X^T X)^{-1} X^T y
\]

Computing \( X^T X \):
\[
X^T X =
\begin{bmatrix}
x_1 & x_2 & \cdots & x_m \\
1 & 1 & \cdots & 1
\end{bmatrix}
\begin{bmatrix}
x_1 & 1 \\
x_2 & 1 \\
\vdots & \vdots \\
x_m & 1 \\
\end{bmatrix}
=
\begin{bmatrix}
\sum_{i=1}^m x_i^2 & \sum_{i=1}^m x_i \\
\sum_{i=1}^m x_i & m
\end{bmatrix}
\]

Now, we compute \( X^T y \):
\[
X^T y =
\begin{bmatrix}
x_1 & x_2 & \cdots & x_m \\
1 & 1 & \cdots & 1
\end{bmatrix}
\begin{bmatrix}
y_1 \\
y_2 \\
\vdots \\
y_m \\
\end{bmatrix}
=
\begin{bmatrix}
\sum_{i=1}^m x_i y_i \\
\sum_{i=1}^m y_i
\end{bmatrix}
\]

Thus, the normal equation becomes:
\[
\theta =
\begin{bmatrix}
\sum_{i=1}^m x_i^2 & \sum_{i=1}^m x_i \\
\sum_{i=1}^m x_i & m
\end{bmatrix}^{-1}
\begin{bmatrix}
\sum_{i=1}^m x_i y_i \\
\sum_{i=1}^m y_i
\end{bmatrix}
\]

Thus,
\[
a = \frac{
m \sum_{i=1}^m x_i y_i - \left( \sum_{i=1}^m x_i \right) \left( \sum_{i=1}^m y_i \right)
}{
m \sum_{i=1}^m x_i^2 - \left( \sum_{i=1}^m x_i \right)^2
}
\]

\[
b = \frac{
\left( \sum_{i=1}^m x_i^2 \right) \left( \sum_{i=1}^m y_i \right)
- \left( \sum_{i=1}^m x_i \right) \left( \sum_{i=1}^m x_i y_i \right)
}{
m \sum_{i=1}^m x_i^2 - \left( \sum_{i=1}^m x_i \right)^2
}
\]

\end{document}